VCVioTest.lean
@@ -9,6 +9,7 @@ public import VCVioTest.MerkleTreeBatch
 public import VCVioTest.MonadProbability
 public import VCVioTest.PFunctorFacade
 public import VCVioTest.ProbabilityTactics
+public import VCVioTest.QueryHom
 public import VCVioTest.RoundByRound.OneRound
 public import VCVioTest.SampleableType
 public import VCVioTest.Smoke
